BoC/Common.lean
@@ -73,14 +73,460 @@ infixr:80 " ∘ "  => Relation.Comp
 postfix:80 " + " => Relation.TransGen
 postfix:80 " * " => Relation.ReflTransGen
 
-/-
-theorem non_empty_middle_inv {A : Type} {l : List A} :
-    List.length l > 0 →
-    ∃ l1 x l2, l = l1 ++ x :: l2 :=
-    by
-    intro h_len
-    cases l with
-    | nil => simp at *
-    | cons hd tl =>
-      exists [], hd, tl
--/
+-- List lemmas
+lemma pair_infix_inv {A} {l : List A} {x1 x2} :
+    [x1, x2] <:+: l →
+    (∃l', l = x1 :: x2 :: l') ∨ [x1, x2] <:+: l.tail :=
+  by
+    introv h_infix
+    rcases h_infix with ⟨init, tail, h_eq⟩
+    subst h_eq
+    cases init with
+    | nil => left; simp
+    | cons y ys =>
+      right; simp
+      exists ys, tail
+      simp
+
+lemma no_dup_pair_eq_r {A} {l : List A} {x1 x2 x3} :
+    List.Pairwise (· ≠ ·) l →
+    [x1, x2] <:+: l →
+    [x1, x3] <:+: l →
+    x2 = x3 :=
+  by
+    introv h_no_dup h_in1 h_in2
+    induction l with
+    | nil =>
+      simp at h_in1
+    | cons y ys h_ih =>
+      simp at h_no_dup
+      rcases h_no_dup with ⟨h_nin, h_no_dup'⟩
+      have h_or1 := pair_infix_inv h_in1
+      have h_or2 := pair_infix_inv h_in2
+      cases h_or1 with
+      | inl h_ex1 =>
+        rcases h_ex1 with ⟨l', h_eq1⟩
+        cases h_or2 with
+        | inl h_ex2 =>
+          rcases h_ex2 with ⟨l'', h_eq2⟩
+          rw [h_eq1] at h_eq2
+          simp at h_eq2
+          exact h_eq2.1
+        | inr h_infix2 =>
+          simp at h_infix2
+          have h_y_eq : y = x1 := by
+            simp at h_eq1
+            exact h_eq1.1
+          have h_x1_nin : x1 ∉ ys := by
+            intro h_mem
+            exact (h_nin x1 h_mem) h_y_eq
+          have h_x1_mem : x1 ∈ ys := by
+            rcases h_infix2 with ⟨init, tail, h_eq⟩
+            rw [← h_eq]
+            simp
+          exfalso
+          exact h_x1_nin h_x1_mem
+      | inr h_infix1 =>
+        cases h_or2 with
+        | inl h_ex2 =>
+          rcases h_ex2 with ⟨l'', h_eq2⟩
+          have h_y_eq : y = x1 := by
+            simp at h_eq2
+            exact h_eq2.1
+          have h_x1_nin : x1 ∉ ys := by
+            intro h_mem
+            exact (h_nin x1 h_mem) h_y_eq
+          simp at h_infix1
+          have h_x1_mem : x1 ∈ ys := by
+            rcases h_infix1 with ⟨init, tail, h_eq⟩
+            rw [← h_eq]
+            simp
+          exfalso
+          exact h_x1_nin h_x1_mem
+        | inr h_infix2 =>
+          exact h_ih h_no_dup' h_infix1 h_infix2
+
+lemma no_dup_pair_eq_l {A} {l : List A} {x1 x2 x3} :
+    List.Pairwise (· ≠ ·) l →
+    [x1, x3] <:+: l →
+    [x2, x3] <:+: l →
+    x1 = x2 :=
+  by
+    introv h_no_dup h_in1 h_in2
+    induction l with
+    | nil =>
+      simp at h_in1
+    | cons y ys h_ih =>
+      simp at h_no_dup
+      rcases h_no_dup with ⟨h_nin, h_no_dup'⟩
+      have h_or := pair_infix_inv h_in1
+      cases h_or with
+      | inl h_ex =>
+        rcases h_ex with ⟨l', h_eq⟩
+        rw [h_eq] at h_in2
+        have h_or' := pair_infix_inv h_in2
+        cases h_or' with
+        | inl h_ex' =>
+          grind
+        | inr h_infix' =>
+          simp at h_infix'
+          simp at h_eq
+          rcases h_eq with ⟨h_eq_y, h_eq_ys⟩
+          subst h_eq_y
+          subst h_eq_ys
+          have h_in : x3 ∈ l' := by
+            rcases h_infix' with ⟨init, tail, h_eq⟩
+            rcases init <;> grind
+          simp at h_no_dup'
+          grind
+      | inr h_infix =>
+        simp at h_infix
+        have h_or' := pair_infix_inv h_in2
+        cases h_or' with
+        | inl h_ex =>
+          rcases h_ex with ⟨l', h_eq⟩
+          simp at h_eq
+          rcases h_eq with ⟨h_eq_y, h_eq_ys⟩
+          subst h_eq_y
+          subst h_eq_ys
+          have h_in : x3 ∈ l' := by
+            rcases h_infix with ⟨init, tail, h_eq⟩
+            rcases init <;> grind
+          simp at h_no_dup'
+          grind
+        | inr h_infix' =>
+          simp at h_infix'
+          grind
+
+lemma pair_sublist_iff {A} {l : List A} {x1 x2} :
+    [x1, x2].Sublist l ↔
+    (∃init mid tail, l = init ++ x1 :: mid ++ x2 :: tail) :=
+  by
+    refine ⟨?_, ?_⟩
+    · introv h_sub
+      induction l with
+      | nil => simp at h_sub
+      | cons y ys =>
+        by_cases h_eq : (y = x1)
+        · subst h_eq
+          rw [List.cons_sublist_cons] at h_sub
+          simp at h_sub
+
+          exists []
+          simp
+          exact List.mem_iff_append.mp h_sub
+        · cases h_sub <;> grind
+    · introv h_ex
+      rcases h_ex with ⟨init, mid, tail, h_eq⟩
+      subst h_eq
+      simp
+
+lemma no_dup_middle_inv {A} {x : A} {l1 l2 l1' l2' : List A} :
+  List.Pairwise (· ≠ ·) (l1 ++ x :: l2) →
+  l1 ++ x :: l2 = l1' ++ x :: l2' →
+  l1 = l1' ∧ l2 = l2' :=
+  by
+    introv h_no_dup h_eq
+    induction l1 generalizing l1' with
+    | nil =>
+      cases l1' with
+      | nil =>
+        simp at h_eq
+        subst h_eq
+        simp
+      | cons a l1'' =>
+        simp at h_eq
+        rcases h_eq with ⟨h_xa, h_rest⟩
+        have h_x_nin : x ∉ l2 := by
+          intro h_mem
+          exact ((List.pairwise_cons.1 h_no_dup).1 x h_mem) rfl
+        have h_x_mem : x ∈ l2 := by
+          rw [h_rest]
+          simp
+        exfalso
+        exact h_x_nin h_x_mem
+    | cons a l1 ih =>
+      cases l1' with
+      | nil =>
+        simp at h_eq
+        rcases h_eq with ⟨h_ax, h_rest⟩
+        have h_a_nin : a ∉ l1 ++ x :: l2 := by
+          intro h_mem
+          exact ((List.pairwise_cons.1 h_no_dup).1 a h_mem) rfl
+        have h_a_mem : a ∈ l1 ++ x :: l2 := by
+          rw [h_ax]
+          simp
+        exfalso
+        exact h_a_nin h_a_mem
+      | cons a' l1'' =>
+        simp at h_eq
+        rcases h_eq with ⟨h_head, h_tail⟩
+        subst h_head
+        have h_no_dup_tail : List.Pairwise (· ≠ ·) (l1 ++ x :: l2) := by
+          simpa [List.cons_append] using (List.pairwise_cons.1 h_no_dup).2
+        rcases ih h_no_dup_tail h_tail with ⟨h_l1, h_l2⟩
+        constructor
+        · simp [h_l1]
+        · exact h_l2
+
+lemma pair_infix_refl_trans_clos_append_left {A} {l1 l2 : List A} {x y} :
+  ((fun e1 e2 ↦ [e1, e2] <:+: l1) *) x y →
+  ((fun e1 e2 ↦ [e1, e2] <:+: l1 ++ l2) *) x y :=
+  by
+    intro h_clos
+    induction h_clos with
+    | refl =>
+      constructor
+    | @tail b c h_clos h_infix ih =>
+      refine Relation.ReflTransGen.tail ih ?_
+      rcases h_infix with ⟨init, tail, h_eq⟩
+      refine ⟨init, tail ++ l2, ?_⟩
+      rw [← h_eq]
+      simp [List.append_assoc]
+
+lemma pair_infix_refl_trans_clos_append_right {A} {l1 l2 : List A} {x y} :
+  ((fun e1 e2 ↦ [e1, e2] <:+: l2) *) x y →
+  ((fun e1 e2 ↦ [e1, e2] <:+: l1 ++ l2) *) x y :=
+  by
+    intro h_clos
+    induction h_clos with
+    | refl =>
+      constructor
+    | @tail b c h_clos h_infix ih =>
+      refine Relation.ReflTransGen.tail ih ?_
+      rcases h_infix with ⟨init, tail, h_eq⟩
+      refine ⟨l1 ++ init, tail, ?_⟩
+      rw [← h_eq]
+      simp [List.append_assoc]
+
+lemma pair_infix_trans_clos_append_left {A} {l1 l2 : List A} {x y} :
+  ((fun e1 e2 ↦ [e1, e2] <:+: l1) +) x y →
+  ((fun e1 e2 ↦ [e1, e2] <:+: l1 ++ l2) +) x y :=
+  by
+    intro h_clos
+    induction h_clos with
+    | @single a h_infix =>
+      apply Relation.TransGen.single
+      rcases h_infix with ⟨init, tail, h_eq⟩
+      refine ⟨init, tail ++ l2, ?_⟩
+      rw [← h_eq]
+      simp [List.append_assoc]
+    | @tail b c h_clos h_infix ih =>
+      refine Relation.TransGen.tail ih ?_
+      rcases h_infix with ⟨init, tail, h_eq⟩
+      refine ⟨init, tail ++ l2, ?_⟩
+      rw [← h_eq]
+      simp [List.append_assoc]
+
+lemma pair_infix_trans_clos_append_right {A} {l1 l2 : List A} {x y} :
+  ((fun e1 e2 ↦ [e1, e2] <:+: l2) +) x y →
+  ((fun e1 e2 ↦ [e1, e2] <:+: l1 ++ l2) +) x y :=
+  by
+    intro h_clos
+    induction h_clos with
+    | @single a h_infix =>
+      apply Relation.TransGen.single
+      rcases h_infix with ⟨init, tail, h_eq⟩
+      refine ⟨l1 ++ init, tail, ?_⟩
+      rw [← h_eq]
+      simp [List.append_assoc]
+    | @tail b c h_clos h_infix ih =>
+      refine Relation.TransGen.tail ih ?_
+      rcases h_infix with ⟨init, tail, h_eq⟩
+      refine ⟨l1 ++ init, tail, ?_⟩
+      rw [← h_eq]
+      simp [List.append_assoc]
+
+lemma pair_infix_clos_middle {A} {x y : A} {mid tail : List A} :
+  ((fun e1 e2 ↦ [e1, e2] <:+: (x :: mid ++ y :: tail))*) x y :=
+  by
+    induction mid generalizing x with
+    | nil =>
+      refine Relation.ReflTransGen.tail (Relation.ReflTransGen.refl) ?_
+      refine ⟨[], tail, ?_⟩
+      simp
+    | cons z zs ih =>
+      have h_tail :
+          ((fun e1 e2 ↦ [e1, e2] <:+: (z :: zs ++ y :: tail))*) z y := by
+        exact ih
+      have h_tail' :
+          ((fun e1 e2 ↦ [e1, e2] <:+: (x :: z :: zs ++ y :: tail))*) z y := by
+        simpa using
+          (pair_infix_refl_trans_clos_append_right
+            (l1 := [x])
+            (l2 := z :: zs ++ y :: tail)
+            h_tail)
+      have h_xz : [x, z] <:+: (x :: z :: zs ++ y :: tail) := by
+        refine ⟨[], zs ++ y :: tail, ?_⟩
+        simp
+      have h_xz_clos :
+          ((fun e1 e2 ↦ [e1, e2] <:+: (x :: z :: zs ++ y :: tail))*) x z := by
+        exact Relation.ReflTransGen.tail (Relation.ReflTransGen.refl) h_xz
+      exact Relation.ReflTransGen.trans h_xz_clos h_tail'
+
+lemma pair_infix_trans_clos_middle {A} {x y : A} {mid tail : List A} :
+  ((fun e1 e2 ↦ [e1, e2] <:+: (x :: mid ++ y :: tail))+) x y :=
+  by
+    induction mid generalizing x with
+    | nil =>
+      apply Relation.TransGen.single
+      refine ⟨[], tail, ?_⟩
+      simp
+    | cons z zs ih =>
+      have h_tail :
+          ((fun e1 e2 ↦ [e1, e2] <:+: (z :: zs ++ y :: tail))+) z y := by
+        exact ih
+      have h_tail' :
+          ((fun e1 e2 ↦ [e1, e2] <:+: (x :: z :: zs ++ y :: tail))+) z y := by
+        simpa using
+          (pair_infix_trans_clos_append_right
+            (l1 := [x])
+            (l2 := z :: zs ++ y :: tail)
+            h_tail)
+      have h_xz : [x, z] <:+: (x :: z :: zs ++ y :: tail) := by
+        refine ⟨[], zs ++ y :: tail, ?_⟩
+        simp
+      exact Relation.TransGen.trans (Relation.TransGen.single h_xz) h_tail'
+
+
+lemma pair_refl_trans_iff {A} {x y : A} {l} :
+  List.Pairwise (· ≠ ·) l →
+  (((fun e1 e2 ↦ [e1, e2] <:+: l)*) x y ↔
+  x = y ∨ List.Sublist [x, y] l) :=
+  by
+    introv h_no_dup
+    refine ⟨?_, ?_⟩
+    · intro h_clos
+      induction h_clos with
+      | refl => simp
+      | @tail b c h_clos h_infix ih =>
+        rcases ih with (h_eq | h_sub)
+        · subst h_eq
+          right
+          exact List.IsInfix.sublist h_infix
+        · right
+          rcases h_infix with ⟨init, tail, h_eq⟩
+          subst h_eq
+          simp at *
+          have h_nin : b ∉ init ∧ b ∉ tail := by
+            rw [List.pairwise_append] at h_no_dup
+            simp at h_no_dup
+            grind
+          rw [pair_sublist_iff] at h_sub
+          rcases h_sub with ⟨init', mid, tail', h_eq'⟩
+          have ⟨h_l1, h_l2⟩ := no_dup_middle_inv (h_no_dup) h_eq'
+          subst h_l1 h_l2
+          grind
+    · intro h_disj
+      cases h_disj with
+      | inl h_eq =>
+        subst h_eq
+        constructor
+      | inr h_sub =>
+        rw [pair_sublist_iff] at h_sub
+        rcases h_sub with ⟨init, mid, tail, h_eq⟩
+        subst h_eq
+        simp [List.append_assoc]
+        apply pair_infix_refl_trans_clos_append_right
+        exact pair_infix_clos_middle
+
+lemma pair_trans_iff {A} {x y : A} {l} :
+  List.Pairwise (· ≠ ·) l →
+  (((fun e1 e2 ↦ [e1, e2] <:+: l)+) x y ↔
+  List.Sublist [x, y] l) :=
+  by
+    introv h_no_dup
+    refine ⟨?_, ?_⟩
+    · intro h_clos
+      induction h_clos with
+      | @single a h_infix =>
+        exact List.IsInfix.sublist h_infix
+      | @tail b c h_clos h_infix ih =>
+        rcases h_infix with ⟨init, tail, h_eq⟩
+        subst h_eq
+        simp at *
+        have h_nin : b ∉ init ∧ b ∉ tail := by
+          rw [List.pairwise_append] at h_no_dup
+          simp at h_no_dup
+          grind
+        rw [pair_sublist_iff] at ih
+        rcases ih with ⟨init', mid, tail', h_eq'⟩
+        have ⟨h_l1, h_l2⟩ := no_dup_middle_inv (h_no_dup) h_eq'
+        subst h_l1 h_l2
+        grind
+    · intro h_sub
+      rw [pair_sublist_iff] at h_sub
+      rcases h_sub with ⟨init, mid, tail, h_eq⟩
+      subst h_eq
+      simp [List.append_assoc]
+      apply pair_infix_trans_clos_append_right
+      exact pair_infix_trans_clos_middle
+
+lemma no_dup_lookup_disjoint {A} {l : List A} {x y : A} {i j : Nat} :
+  List.Pairwise (· ≠ ·) l →
+  l[i]? = some x →
+  l[j]? = some y →
+  i ≠ j →
+  x ≠ y :=
+  by
+    introv h_no_dup h_lookup_i h_lookup_j h_neq
+    induction l generalizing i j x y with
+    | nil =>
+      simp at h_lookup_i
+    | cons a l ih =>
+      rcases (List.pairwise_cons.1 h_no_dup) with ⟨h_notin, h_no_dup'⟩
+      cases i with
+      | zero =>
+        simp at h_lookup_i
+        subst h_lookup_i
+        cases j with
+        | zero =>
+          exfalso
+          contradiction
+        | succ j =>
+          simp at h_lookup_j
+          intro h_eq
+          subst h_eq
+          have h_mem_a : a ∈ l := by
+            exact (List.mem_iff_getElem?).2 ⟨j, h_lookup_j⟩
+          grind
+      | succ i =>
+        simp at h_lookup_i
+        cases j with
+        | zero =>
+          simp at h_lookup_j
+          intro h_eq
+          have h_mem_a : x ∈ l := (List.mem_iff_getElem?).2 ⟨i, h_lookup_i⟩
+          grind
+        | succ j =>
+          simp at h_lookup_j
+          apply ih h_no_dup' h_lookup_i h_lookup_j
+          intro h_eq
+          subst h_eq
+          contradiction
+
+lemma list_snoc_cases {A} {l : List A} :
+  l = [] ∨ ∃l' x, l = l' ++ [x] :=
+  by
+    induction l with
+    | nil => simp
+    | cons y ys ih =>
+      simp
+      cases ih with
+      | inl h_eq =>
+        subst h_eq
+        exists [], y
+      | inr h_snoc =>
+        rcases h_snoc with ⟨l', x, h_eq⟩
+        subst h_eq
+        exists (y :: l'), x
+
+lemma list_snoc_eq_inv {A} {l1 l2 : List A} {x1 x2 : A} :
+  l1 ++ [x1] = l2 ++ [x2] →
+  (l1 = l2 ∧ x1 = x2) :=
+  by
+    simp
+
+def bad_example : Prop := 3 < 2
+-- ∃n∈N. 5 < n ∧ n<10
+def example2 := ∃n : ℕ, 5 < n ∧ n < 10
